AVL.fst
@@ -88,10 +88,48 @@ let rec find_max #a (#f: comparaison a) (input: set f{Node? input}) : a =
     | Node l k h Leaf -> k
     | Node l k _ r -> find_max r
 
+let rec remove #a (#f: comparaison a) (x:a) (input:set f): Tot (out: set f) (decreases input) = 
+
+
+    match input with 
+    | Leaf -> input
+    | Node l k _ r -> match f x k with 
+        | LT -> 
+        begin 
+            let l' = remove x l in
+            if Node? r && delta l' r >= 2 then begin
+                if height (left r) > height (right r) 
+                then balanceRL l' k r
+                else balanceRR l' k r
+            end else make l' k r
+        end 
+        | GT -> 
+        begin
+            let r' = remove x r in 
+            if Node? l && delta l r' >= 2 then begin 
+                if height (left l) < height (right l) 
+                then balanceLR l k r' 
+                else balanceLL l k r'
+            end else make l k r'
+        end 
+        | EQ -> 
+            if Leaf? l then r else 
+            if Leaf? r then l else begin
+
+            let k' = find_min r in 
+            let r' = remove k' r in
+            
+            if delta l r' >= 2 then begin 
+                if height (left l) < height (right l) 
+                then balanceLR l k' r' 
+                else balanceLL l k' r'
+            end else make l k' r'
+            
+        end 
 
 (* proof *)
 
-#push-options "--z3rlimit 60"
+#push-options "--z3rlimit 50"
 
 
 let rec find_min_lemma #a (#f: comparaison a) (input: set f{Node? input}) : 
@@ -104,7 +142,6 @@ let rec find_min_lemma #a (#f: comparaison a) (input: set f{Node? input}) :
      = match input with 
     | Node Leaf k h r -> ()
     | Node l k _ r -> find_min_lemma l
-    | Leaf -> ()
 
 let rec find_max_lemma #a (#f: comparaison a) (input: set f{Node? input}) : 
     Lemma 
@@ -116,7 +153,6 @@ let rec find_max_lemma #a (#f: comparaison a) (input: set f{Node? input}) :
      = match input with 
     | Node l k h Leaf -> ()
     | Node l k _ r -> find_max_lemma r
-    | Leaf -> ()
 
 
 private let balanceLL_lemma #a (#f: comparaison a) (l: set f{Node? l}) (k:a) (r:set f) : 
@@ -277,71 +313,6 @@ let rec add_lemma #a (#f: comparaison a) (x:a) (input:set f):
                 else balanceRR_lemma l k r' 
             end else make_lemma l k r' 
         end 
-
-
-
-
-let rec remove #a (#f: comparaison a) (x:a) (input:set f{is_avl input}): out:set f{        
-        
-        (forall y. (member y input /\ ~(EQ? (f x y))) <==> member y out) /\ 
-        is_avl out /\ height out <= height input /\ 
-        height out >= height input - 1
-    } = 
-    
-    match input with 
-    | Leaf -> input
-    | Node l k _ r -> match f x k with 
-        | LT -> 
-        begin 
-            let l' = remove x l in 
-            if delta l' r >= 2 then begin 
-                if height (left r) > height (right r) 
-                then begin balanceRL_lemma l' k r; balanceRL l' k r end 
-                else begin 
-                    if delta (left r) (right r) = 0
-                    then balanceRR_lemma2 l' k r 
-                    else balanceRR_lemma  l' k r
-                    ; balanceRR l' k r
-                end 
-            end else make l' k r
-        end 
-        | GT -> 
-        begin
-            let r' = remove x r in 
-            if delta l r' >= 2 then begin 
-                assert (height l >= 2); 
-                if height (left l) < height (right l) 
-                then begin balanceLR_lemma l k r'; balanceLR l k r' end
-                else begin 
-                    if delta (left l) (right l) = 0 
-                    then balanceLL_lemma2 l k r'
-                    else balanceLL_lemma  l k r'
-                    ; balanceLL l k r'
-                end 
-            end else make l k r'
-        end 
-        | EQ -> 
-        begin 
-            admit() (*
-            match l, r with 
-            | Leaf, _ -> r 
-            | _, Leaf -> l 
-            | l, r -> begin 
-            find_min_lemma r; 
-            let k' = find_min r in 
-            let r' = remove k' r in 
-            if delta l r' >= 2 then begin
-                assert (height l >= 2); 
-                if height (left l) < height (right l) 
-                then admit()//balanceLR l k' r'
-                else admit()//balanceLL l k' r' 
-            end else make l k' r'
-            end *)
-        end
-
-
-
-
 
 
 
